Improve correspondence proof axiomatic <-> small step semantics.

axiomatic.v
@@ -8,7 +8,7 @@ Definition dassert_pack (Ψ : (label → assert) * (option N → assert))
     (P : assert) (Q: assert) : direction → assert :=
   direction_rect (λ _, assert) P Q (snd Ψ) (fst Ψ).
 
-Instance: Proper 
+Lemma dassert_pack_proper: Proper 
   (prod_relation (pointwise_relation _ (≡)) (pointwise_relation _ (≡)) ==>
     (≡) ==> (≡) ==> (=) ==> (≡)) dassert_pack.
 Proof. intros ?????????? d ?. subst. destruct d; firstorder. Qed.
@@ -18,29 +18,33 @@ Definition dassert_map (f : assert → assert) (P : dassert) : dassert :=
 Lemma dassert_map_spec f P d : dassert_map f P d = f (P d).
 Proof. now destruct d. Qed.
 
-Inductive ax_conclusion (P : dassert) (k : ctx) (mr : mem) (S : state) : Prop :=
-  | ax_further ml :
-     mem_disjoint ml mr →
-     SMem S = ml ∪ mr →
-     red (⇨{k}) S →
-     ax_conclusion P k mr S
-  | ax_done ml :
-     mem_disjoint ml mr →
-     SMem S = ml ∪ mr →
-     SCtx S = k →
-     up (SDir S) (SStmt S) →
-     P (SDir S) (get_stack k) ml →
-     ax_conclusion P k mr S.
+Inductive ax_stmt_conclusion (P : dassert) (s : stmt) (k : ctx) (mr : mem) : state → Prop :=
+  | ax_stmt_further ml' d' k' s' :
+     mem_disjoint ml' mr →
+     red (⇨{k}) (State d' k' s' (ml' ∪ mr)) →
+     ax_stmt_conclusion P s k mr (State d' k' s' (ml' ∪ mr))
+  | ax_stmt_done ml' d :
+     mem_disjoint ml' mr →
+     up d s →
+     P d (get_stack k) ml'  →
+     ax_stmt_conclusion P s k mr (State d k s (ml' ∪ mr)).
 
-Definition ax (s : stmt) (P : dassert) := ∀ d k ml mr S',
+Definition ax_stmt (s : stmt) (P : dassert) := ∀ d k ml mr S',
     mem_disjoint ml mr →
     State d k s (ml ∪ mr) ⇨{k}* S' →
     down d s →
     P d (get_stack k) ml →
-  ax_conclusion P k mr S'.
-Notation "Ψ ⊢ ⦃ P ⦄ s ⦃ Q ⦄" := (ax s%S (dassert_pack Ψ%A P%A Q%A)) (at level 80).
+  ax_stmt_conclusion P s k mr S'.
+Notation "Ψ ⊢ ⦃ P ⦄ s ⦃ Q ⦄" := (ax_stmt s%S (dassert_pack Ψ%A P%A Q%A)) (at level 80).
 
-Lemma ax_split s P (Hax : ax s P) l n d k ml mr S'' :
+Ltac my_inversion H IP :=
+  match type of H with
+  | ?T1 → ?T2 => let H' := fresh in assert T1 as H'; [ | my_inversion (H H') IP; clear H' ]
+  | _ => let H' := fresh in pose proof H as H'; inversion H' as IP; clear H'
+  end.
+Tactic Notation "my_inversion" constr(H) "as" simple_intropattern(IP) := my_inversion H IP.
+
+Lemma ax_stmt_split s P (Hax : ax_stmt s P) l n d k ml mr S'' :
     mem_disjoint ml mr →
     State d (l ++ k) s (ml ∪ mr) ⇨{k}^n S'' →
     down d s →
@@ -55,29 +59,20 @@ Lemma ax_split s P (Hax : ax s P) l n d k ml mr S'' :
     ∧ n' ≤ n
     ∧ up d' s ∧ P d' (get_stack l ++ get_stack k) ml').
 Proof.
-  intros ? p1 Hdown HP.
+  intros ? p1 ??.
   rewrite <-get_stack_app in *.
   destruct (cstep_subctx_cut l k _ _ _ p1)
     as [? | [n' [S' [p2 [p3 [??]]]]]]; eauto with list.
-   destruct (Hax d (l ++ k) ml mr S'') as [ml'' | ml'']; auto.
-    left. exists ml''. now auto.
-   destruct S'' as [d'' k'' s'' m'']; simpl in *.
-   right. exists 0 d'' ml''.
-   assert (s = s''); subst.
-    eapply csteps_preserve_stmt.
-    now apply (rtc_subrel (⇨{l ++ k}) (⇨) _); eauto.
-   now intuition.
-  right. destruct (Hax d (l ++ k) ml mr S') as [ml' | ml']; auto.
-   exists n' (SDir S') ml'. now auto.
-  destruct S' as [d' k' s' m']; simpl in *.
-  assert (s = s'); subst.
-   eapply csteps_preserve_stmt.
-   now apply (rtc_subrel (⇨{l ++ k}) (⇨) _); eauto.
-  exists n' d' ml'. now auto.
+   my_inversion (Hax d (l ++ k) ml mr S'') as [ml'' | ml'' d'']; subst; auto.
+    left. exists ml''. simpl. now auto.
+   right. exists 0 d'' ml''. intuition.
+  my_inversion (Hax d (l ++ k) ml mr S') as [ml' | ml' d']; subst; auto.
+   contradiction.
+  right. exists n' d' ml'. now auto.
 Qed.
 
-Lemma ax_sound s P d m d' k' s' m' :
-  ax s P →
+Lemma ax_stmt_sound s P d m d' k' s' m' :
+  ax_stmt s P →
     State d [] s m ⇨* State d' k' s' m' →
     nf (⇨) (State d' k' s' m') →
     down d s →
@@ -87,38 +82,46 @@ Lemma ax_sound s P d m d' k' s' m' :
   ∧ P d' [] m'.
 Proof.
   intros Hax p Hnf ??.
-  destruct (Hax d [] m ∅ (State d' k' s' m')) as [m'' | m'']; auto.
+  my_inversion (Hax d [] m ∅ (State d' k' s' m')) as [m'' | m'']; subst; auto.
   * auto with mem.
   * rewrite (right_id ∅ _). now apply (rtc_subrel (⇨) (⇨{[]}) _).
   * destruct Hnf. now apply (red_subrel (⇨{[]}) _ _).
   * simpl in *. subst. rewrite (right_id ∅ _). now auto.
 Qed.
 
-Lemma ax_weak Ψ P Q s : 
-  Ψ ⊢ ⦃ P ⦄ s ⦃ Q ⦄ → ∀ P' Q', P' ⊆ P → Q ⊆ Q' → Ψ ⊢ ⦃ P' ⦄ s ⦃ Q' ⦄.
+Lemma ax_stmt_weak_packed Ppack Ppack' s :
+  (∀ d, down d s → (Ppack' d → Ppack d)%A) →
+  (∀ d, up d s → (Ppack d → Ppack' d)%A) →
+  ax_stmt s Ppack → ax_stmt s Ppack'.
 Proof.
-  intros Hax P' Q' HP HQ d k ml mr S' ????.
-  destruct (Hax d k ml mr S') as [ml' | ml']; auto.
-    now destruct d; intuition.
-   now left with ml'.
-  right with ml'; auto. destruct (SDir S'); intuition.
+  intros Hdown Hup Hax d k ml mr S' ????.
+  my_inversion (Hax d k ml mr S') as [ml' | ml' d']; subst; auto.
+  * now apply Hdown.
+  * now left.
+  * right; auto. now apply Hup.
 Qed.
 
+Lemma ax_stmt_weak_pre Ψ P P' Q s : 
+  P' ⊆ P → Ψ ⊢ ⦃ P ⦄ s ⦃ Q ⦄ → Ψ ⊢ ⦃ P' ⦄ s ⦃ Q ⦄.
+Proof. intro. apply ax_stmt_weak_packed; intros []; solve_assert. Qed.
+Lemma ax_stmt_weak_post Ψ P Q Q' s : 
+  Q ⊆ Q' → Ψ ⊢ ⦃ P ⦄ s ⦃ Q ⦄ → Ψ ⊢ ⦃ P ⦄ s ⦃ Q' ⦄.
+Proof. intro. apply ax_stmt_weak_packed; intros []; solve_assert. Qed.
+
 Lemma ax_frame_packed A Ppack s :
-  ax s Ppack → ax s (dassert_map (λ P, P * A)%A Ppack).
+  ax_stmt s Ppack → ax_stmt s (dassert_map (λ P, P * A)%A Ppack).
 Proof.
-  intros Hax d k m1 m4 S' ???.
+  intros Hax d k m1 m4 S' ? p ?.
   rewrite dassert_map_spec.
   intros [m2 [m3 [? [? [??]]]]]. subst.
-  destruct (Hax d k m2 (m3 ∪ m4) S') as [ml2' | ml2']; auto.
+  my_inversion (Hax d k m2 (m3 ∪ m4) S') as [ml2' | ml2']; subst; auto.
      solve_mem_disjoint.
-    now rewrite (associative _).
-   left with (ml2' ∪ m3); auto.
+    now rewrite (associative_eq _).
+   rewrite (associative_eq _). left.
     solve_mem_disjoint.
-   now rewrite <-(associative _).
-  right with (ml2' ∪ m3); auto.
-    solve_mem_disjoint.
-   now rewrite <-(associative _).
+   now rewrite <-(associative_eq _).
+  rewrite (associative_eq _). right; auto.
+   solve_mem_disjoint.
   rewrite dassert_map_spec.
   exists ml2' m3. intuition. solve_mem_disjoint.
 Qed.
@@ -131,33 +134,32 @@ Lemma ax_and Ψ P Q Q' s :
   Ψ ⊢ ⦃ P ⦄ s ⦃ Q ⦄ → Ψ ⊢ ⦃ P ⦄ s ⦃ Q' ⦄ → Ψ ⊢ ⦃ P ⦄ s ⦃ Q ∧ Q' ⦄.
 Proof.
   intros Hax1 Hax2 d k ml mr S' ??? Hpre.
-  destruct (Hax1 d k ml mr S') as [ml' | ml']; auto.
+  my_inversion (Hax1 d k ml mr S') as [ml' | ml' d']; subst; auto.
     now destruct d; intuition.
-   now left with ml'.
-  destruct (Hax2 d k ml mr S') as [ml'' | ml'']; auto.
+   now left.
+  my_inversion (Hax2 d k ml mr (State d' k s (ml' ∪ mr))) as [ml'' | ml'']; subst; auto.
     now destruct d; intuition.
-   now left with ml'.
+   left. easy. congruence.
   assert (ml' = ml''); subst.
    now apply mem_union_cancel_l with mr; intuition congruence.
-  right with ml''; auto.
-  destruct (SDir S'); intuition auto. now split.
+  right; auto. destruct d'; intuition auto. now split.
 Qed.
 
 Lemma ax_skip Ψ P : Ψ ⊢ ⦃ P ⦄ skip ⦃ P ⦄.
 Proof.
   intros d k ml mr S' ? p ??. inv_csteps p as [ | ???? p].
-   left with ml; auto. solve_cnf.
+   left. easy. solve_cnf.
   inv_cstep. inv_csteps p; simpl in *.
-   now right with ml.
+   now right.
   inv_cstep.
 Qed.
 
 Lemma ax_goto Ψ Q l : Ψ ⊢ ⦃ fst Ψ l ⦄ goto l ⦃ Q ⦄.
 Proof.
   intros d k ml mr S' ? p ??. inv_csteps p as [ | ???? p].
-   left with ml; auto. solve_cnf.
+   left. easy. solve_cnf.
   inv_cstep. inv_csteps p; simpl in *.
-   right with ml; auto. simplify_elem_of.
+   right; simplify_elem_of.
   inv_cstep.
 Qed.
 
@@ -167,10 +169,9 @@ Proof.
   destruct d; try contradiction.
   destruct Hpre as [v [??]]. simplify_assert_expr.
   inv_csteps p as [| ???? p ]; simpl in *.
-   left with ml; auto. solve_cnf.
+   left. easy. solve_cnf.
   inv_cstep. inv_csteps p; simpl in *.
-   simplify_assert_expr.
-   now right with ml.
+   simplify_assert_expr. now right.
   inv_cstep.
 Qed.
 
@@ -180,8 +181,7 @@ Proof.
   intros d k ml mr S' ? p ? Hpre.
   destruct d; try contradiction.
   inv_csteps p as [| ???? p ]; simpl in *.
-   left with ml; auto.
-   destruct Hpre as [a [v [? [? [[??] ?]]]]].
+   left. easy. destruct Hpre as [a [v [? [? [[??] ?]]]]].
    simplify_assert_expr.
    assert (is_writable a (ml ∪ mr)).
     do 2 red. eauto with mem.
@@ -189,9 +189,8 @@ Proof.
   inv_cstep. inv_csteps p; simpl in *.
    destruct Hpre as [a' [v' [? [? [[??] ?]]]]].
    simplify_assert_expr.
-   right with (<[a:=v]>ml); auto.
-    now eauto with mem.
-   now rewrite mem_union_insert_l.
+   rewrite mem_union_insert_l.
+   right; eauto with mem.
   inv_cstep.
 Qed.
 
@@ -204,23 +203,23 @@ Proof.
       State d (CItem (loop □) :: k) s (ml ∪ mr) ⇨{k}^n S5 →
       down d s →
       dassert_pack Ψ P P d (get_stack k) ml →
-    ax_conclusion (dassert_pack Ψ P Q) k mr S5).
+    ax_stmt_conclusion (dassert_pack Ψ P Q) (loop s) k mr S5).
    induction n as [n1 IH] using lt_wf_ind.
    intros d1 ml1 ? p1 ??.
-   edestruct (ax_split s _ Hax [CItem (loop □)])
+   edestruct (ax_stmt_split s _ Hax [CItem (loop □)])
      as [[ml2 [? [??]]] | [n' [d2 [ml2 [? [p2 ?]]]]]]; simpl in *; eauto.
-    left with ml2; auto. solve_cnf.
+    destruct S5; simpl in *; subst. left. easy. solve_cnf.
    inv_csteps p2 as [| n3 ? S3 ? p2 p3]; simpl in *.
-    left with ml2; auto. solve_cnf.
+    left. easy. solve_cnf.
    { inv_cstep p2; try solve [simplify_stmt_elem_of].
    * inv_csteps p3 as [| n4 ? S4 ? p3 p4]; simpl in *.
-       left with ml2; auto. solve_cnf.
+       left. easy. solve_cnf.
       inv_cstep. eapply (IH n4); intuition eauto. omega.
-   * inv_csteps p3; simpl in *. now right with ml2. inv_cstep.
-   * inv_csteps p3; simpl in *. now right with ml2. inv_cstep. }
+   * inv_csteps p3; simpl in *. now right. inv_cstep.
+   * inv_csteps p3; simpl in *. now right. inv_cstep. }
   intros d ml ? p ??.
   destruct (rtc_nsteps p) as [n pn]. inv_csteps pn; simpl in*.
-   left with ml; auto. solve_cnf.
+   left. easy. solve_cnf.
   inv_cstep; eauto.
 Qed.
 
@@ -234,28 +233,27 @@ Proof.
       State d (CItem (l :; □) :: k) s (ml ∪ mr) ⇨{k}^n S5 →
       down d s →
       dassert_pack Ψ (fst Ψ l) Q d (get_stack k) ml →
-    ax_conclusion (dassert_pack Ψ (fst Ψ l) Q) k mr S5).
+    ax_stmt_conclusion (dassert_pack Ψ (fst Ψ l) Q) (l :; s) k mr S5).
    induction n as [n1 IH] using lt_wf_ind.
    intros d1 ml1 ? p1 ??.
-   edestruct (ax_split s _ Hax [CItem (l :; □)])
+   edestruct (ax_stmt_split s _ Hax [CItem (l :; □)])
      as [[ml2 [? [??]]] | [n' [d2 [ml2 [? [p2 ?]]]]]]; simpl in *; eauto.
-    left with ml2; auto. solve_cnf.
+    destruct S5; simpl in *; subst. left. easy. solve_cnf.
    inv_csteps p2 as [| n3 ? S3 ? p2 p3]; simpl in *.
-    left with ml2; auto. solve_cnf.
+    left. easy. solve_cnf.
    { inv_cstep p2; try solve [simplify_stmt_elem_of].
-   * inv_csteps p3; simpl in *. now right with ml2. inv_cstep.
-   * inv_csteps p3; simpl in *. now right with ml2. inv_cstep.
+   * inv_csteps p3; simpl in *. now right. inv_cstep.
+   * inv_csteps p3; simpl in *. now right. inv_cstep.
    * match goal with
-     | _ : State (Goto ?l') _ _ _ ⇨{_}^_ _ |- _ => destruct (decide (l' = l))
+     | _ : ?l' ∉ labels s |- _ => destruct (decide (l' = l))
      end; simpl in *; subst.
     + inv_csteps p3 as [| n4 ? S4 ? p3 p4]; simpl in *.
-         left with ml2; auto. solve_cnf.
+         left. easy. solve_cnf.
         inv_cstep. eapply (IH n4); intuition eauto. omega.
-    + inv_csteps p3; simpl in *. right with ml2; simplify_elem_of. inv_cstep. }
+    + inv_csteps p3; simpl in *. right; simplify_elem_of. inv_cstep. }
   intros d ml ? p ??.
   destruct (rtc_nsteps p) as [n pn]. inv_csteps pn; simpl in *.
-   left with ml; auto.
-   destruct d; simplify_elem_of; solve_cnf. 
+   left. easy. destruct d; simplify_elem_of; solve_cnf. 
   inv_cstep; eauto.
 Qed.
 
@@ -274,43 +272,42 @@ Proof.
     ∨ (State d (CItem (sl ;; □) :: k) sr (ml ∪ mr) ⇨{k}^n S5
       ∧ down d sr
       ∧ dassert_pack Ψ P' Q d (get_stack k) ml) →
-    ax_conclusion (dassert_pack Ψ P Q) k mr S5).
+    ax_stmt_conclusion (dassert_pack Ψ P Q) (sl ;; sr) k mr S5).
    induction n as [n IH] using lt_wf_ind.
    intros d1 ml1 ? [[p1 [??]] | [p1 [??]]].
-    edestruct (ax_split sl _ Haxl [CItem (□ ;; sr)])
+    edestruct (ax_stmt_split sl _ Haxl [CItem (□ ;; sr)])
       as [[ml2 [? [??]]] | [n' [d2 [ml2 [? [p2 ?]]]]]]; simpl in *; eauto.
-     left with ml2; auto. solve_cnf.
+     destruct S5; simpl in *; subst. left. easy. solve_cnf.
     inv_csteps p2 as [| n3 ? S3 ? p2 p3]; simpl in *.
-     left with ml2; auto. solve_cnf.
+     left. easy. solve_cnf.
     { inv_cstep p2; try solve [simplify_stmt_elem_of].
     * eapply (IH n3); intuition eauto.
-    * inv_csteps p3; simpl in *. now right with ml2. inv_cstep.
+    * inv_csteps p3; simpl in *. now right. inv_cstep.
     * match goal with
-     | _ : State (Goto ?l') _ _ _ ⇨{_}^_ _ |- _ => destruct (decide (l ∈ labels sr))
+     | _ : ?l ∉ labels sl |- _ => destruct (decide (l ∈ labels sr))
      end; simpl in *; subst.
      + inv_csteps p3 as [| n4 ? S4 ? p3 p4]; simpl in *.
-          left with ml2; auto. solve_cnf.
+          left. easy. solve_cnf.
          inv_cstep. eapply (IH n4); intuition eauto. omega.
-     + inv_csteps p3; simpl in *. right with ml2; simplify_elem_of. inv_cstep. }
-   edestruct (ax_split sr _ Haxr [CItem (sl ;; □)])
+     + inv_csteps p3; simpl in *. right; simplify_elem_of. inv_cstep. }
+   edestruct (ax_stmt_split sr _ Haxr [CItem (sl ;; □)])
      as [[ml2 [? [??]]] | [n' [d2 [ml2 [? [p2 ?]]]]]]; simpl in *; eauto.
-    left with ml2; auto. solve_cnf.
+    destruct S5; simpl in *; subst. left. easy. solve_cnf.
    inv_csteps p2 as [| n3 ? S3 ? p2 p3]; simpl in *.
-    left with ml2; auto. solve_cnf.
+    left. easy. solve_cnf.
    { inv_cstep p2; try solve [simplify_stmt_elem_of].
-   * inv_csteps p3; simpl in *. now right with ml2. inv_cstep.
-   * inv_csteps p3; simpl in *. now right with ml2. inv_cstep.
+   * inv_csteps p3; simpl in *. now right. inv_cstep.
+   * inv_csteps p3; simpl in *. now right. inv_cstep.
    * match goal with
-    | _ : State (Goto ?l') _ _ _ ⇨{_}^_ _ |- _ => destruct (decide (l ∈ labels sl))
+    | _ : ?l ∉ labels sr |- _ => destruct (decide (l ∈ labels sl))
     end; simpl in *; subst.
     + inv_csteps p3 as [| n4 ? S4 ? p3 p4]; simpl in *.
-         left with ml2; auto. solve_cnf.
+         left. easy. solve_cnf.
         inv_cstep. eapply (IH n4); intuition eauto. omega.
-    + inv_csteps p3; simpl in *. right with ml2; simplify_elem_of. inv_cstep. }
+    + inv_csteps p3; simpl in *. right; simplify_elem_of. inv_cstep. }
   intros d ml ? p ??.
   destruct (rtc_nsteps p) as [n pn]. inv_csteps pn; simpl in *.
-   left with ml; auto.
-   destruct d; simplify_elem_of; solve_cnf. 
+   left. easy. destruct d; simplify_elem_of; solve_cnf. 
   inv_cstep; eauto.
 Qed.
 
@@ -329,55 +326,54 @@ Proof.
     ∨ (State d (CItem (IF e then sl else □) :: k) sr (ml ∪ mr) ⇨{k}^n S5
       ∧ down d sr
       ∧ dassert_pack Ψ (P ∧ ∃ v, e⇓v ∧ ⌜ val_false v ⌝)%A Q d (get_stack k) ml) →
-    ax_conclusion (dassert_pack Ψ (P ∧ e⇓-)%A Q) k mr S5) as help.
+    ax_stmt_conclusion (dassert_pack Ψ (P ∧ e⇓-) Q) (IF e then sl else sr) k mr S5) as help.
    induction n as [n IH] using lt_wf_ind.
    intros d1 ml1 ? [[p1 [??]] | [p1 [??]]].
-    edestruct (ax_split sl _ Haxl [CItem (IF e then □ else sr)])
+    edestruct (ax_stmt_split sl _ Haxl [CItem (IF e then □ else sr)])
       as [[ml2 [? [??]]] | [n' [d2 [ml2 [? [p2 ?]]]]]]; simpl in *; eauto.
-     left with ml2; auto. solve_cnf.
+     destruct S5; simpl in *; subst. left. easy. solve_cnf.
     inv_csteps p2 as [| n3 ? S3 ? p2 p3]; simpl in *.
-     left with ml2; auto. solve_cnf.
+     left. easy. solve_cnf.
     { inv_cstep p2; try solve [simplify_stmt_elem_of].
-    * inv_csteps p3; simpl in *. now right with ml2. inv_cstep.
-    * inv_csteps p3; simpl in *. now right with ml2. inv_cstep.
+    * inv_csteps p3; simpl in *. now right. inv_cstep.
+    * inv_csteps p3; simpl in *. now right. inv_cstep.
     * match goal with
-     | _ : State (Goto ?l') _ _ _ ⇨{_}^_ _ |- _ => destruct (decide (l ∈ labels sr))
+     | _ : ?l ∉ labels sl |- _ => destruct (decide (l ∈ labels sr))
      end; simpl in *; subst.
      + inv_csteps p3 as [| n4 ? S4 ? p3 p4]; simpl in *.
-          left with ml2; auto. solve_cnf.
+          left. easy. solve_cnf.
          inv_cstep. eapply (IH n4); intuition eauto. omega.
-     + inv_csteps p3; simpl in *. right with ml2; simplify_elem_of. inv_cstep. }
-   edestruct (ax_split sr _ Haxr [CItem (IF e then sl else □)])
+     + inv_csteps p3; simpl in *. right; simplify_elem_of. inv_cstep. }
+   edestruct (ax_stmt_split sr _ Haxr [CItem (IF e then sl else □)])
      as [[ml2 [? [??]]] | [n' [d2 [ml2 [? [p2 ?]]]]]]; simpl in *; eauto.
-    left with ml2; auto. solve_cnf.
+    destruct S5; simpl in *; subst. left. easy. solve_cnf.
    inv_csteps p2 as [| n3 ? S3 ? p2 p3]; simpl in *.
-    left with ml2; auto. solve_cnf.
+    left. easy. solve_cnf.
    { inv_cstep p2; try solve [simplify_stmt_elem_of].
-   * inv_csteps p3; simpl in *. now right with ml2. inv_cstep.
-   * inv_csteps p3; simpl in *. now right with ml2. inv_cstep.
+   * inv_csteps p3; simpl in *. now right. inv_cstep.
+   * inv_csteps p3; simpl in *. now right. inv_cstep.
    * match goal with
-    | _ : State (Goto ?l') _ _ _ ⇨{_}^_ _ |- _ => destruct (decide (l ∈ labels sl))
+    | _ : ?l ∉ labels sr |- _ => destruct (decide (l ∈ labels sl))
     end; simpl in *; subst.
     + inv_csteps p3 as [| n4 ? S4 ? p3 p4]; simpl in *.
-         left with ml2; auto. solve_cnf.
+         left. easy. solve_cnf.
         inv_cstep. eapply (IH n4); intuition eauto. omega.
-    + inv_csteps p3; simpl in *. right with ml2; simplify_elem_of. inv_cstep. }
+    + inv_csteps p3; simpl in *. right; simplify_elem_of. inv_cstep. }
   intros d ml ? p ? Hpre.
-  destruct (rtc_nsteps p) as [n pn].
+  destruct (rtc_nsteps p) as [n pn]. clear p.
   destruct d; simpl in *; try contradiction.
   * destruct Hpre as [? [v ?]].
      inv_csteps pn; simpl in *.
-      left with ml; auto.
-      destruct (val_true_false_dec v); solve_cnf.
+      left. easy. destruct (val_true_false_dec v); solve_cnf.
      inv_cstep; simplify_assert_expr; eapply help; eauto;
        [left | right]; clear help Haxl Haxr; solve_assert.
   * inv_csteps pn; simpl in *.
-      left with ml; auto. simplify_elem_of; solve_cnf.
+      left. easy. simplify_elem_of; solve_cnf.
      inv_cstep; eauto.
 Qed.
 
 Lemma ax_block_packed Ppack s :
-  ax s (dassert_map (λ P, P↑* (O↦ -))%A Ppack) → ax (SBlock s) Ppack.
+  ax_stmt s (dassert_map (λ P, P↑* (O↦ -))%A Ppack) → ax_stmt (SBlock s) Ppack.
 Proof.
   intros Hax d k ml mr S5 Hdisjoint p1.
   revert d ml Hdisjoint p1.
@@ -387,32 +383,28 @@ Proof.
       State d (CBlock b :: k) s (<[b:=v]>(ml ∪ mr)) ⇨{k}^n S5 →
       down d s →
       Ppack d (get_stack k) ml →
-    ax_conclusion Ppack k mr S5).
+    ax_stmt_conclusion Ppack (SBlock s) k mr S5).
    intros n d1 ml1 b v Hdisjoint Hfree p1 ??.
-   rewrite mem_union_insert_l in p1.
-   red in Hfree. rewrite mem_union_None_iff in Hfree. destruct Hfree.
-   assert (mem_disjoint (<[ b:=v ]>ml1) mr).
-    apply mem_disjoint_insert_l; auto.
-   clear Hdisjoint.
-   edestruct (ax_split s _ Hax [CBlock b])
+   setoid_rewrite mem_union_None_iff in Hfree. destruct Hfree.
+   assert (mem_disjoint (<[ b:=v ]>ml1) mr) by eauto with mem.
+   edestruct (ax_stmt_split s _ Hax [CBlock b])
      as [[ml2 [? [??]]] | [n' [d2 [ml2 [? [p2 [? [? Hpost]]]]]]]]; simpl in *; eauto.
-     rewrite dassert_map_spec.
-     apply assert_alloc; auto.
-    left with ml2; auto. solve_cnf.
-   rewrite dassert_map_spec in Hpost.
-   apply assert_free in Hpost.
-   assert (delete b (ml2 ∪ mr) = delete b ml2 ∪ mr).
+      rewrite <-mem_union_insert_l; eauto.
+     rewrite dassert_map_spec. auto using assert_alloc.
+    destruct S5; simpl in *; subst. left. easy. solve_cnf.
+   rewrite dassert_map_spec in Hpost. apply assert_free in Hpost.
+   assert (delete b (ml2 ∪ mr) = delete b ml2 ∪ mr) as Em.
     now rewrite mem_union_delete, (delete_lookup_None mr).
    inv_csteps p2 as [| n3 ? S3 ? p2 p3]; simpl in *.
-    left with ml2; auto. solve_cnf.
+    left. easy. solve_cnf.
    { inv_cstep p2; try solve [simplify_stmt_elem_of].
-   * inv_csteps p3; simpl in *. right with (delete b ml2); auto with mem. inv_cstep.
-   * inv_csteps p3; simpl in *. right with (delete b ml2); auto with mem. inv_cstep.
-   * inv_csteps p3; simpl in *. right with (delete b ml2); auto with mem. inv_cstep. }
+   * inv_csteps p3; simpl in *. rewrite Em. right; auto with mem. inv_cstep.
+   * inv_csteps p3; simpl in *. rewrite Em. right; auto with mem. inv_cstep.
+   * inv_csteps p3; simpl in *. rewrite Em. right; auto with mem. inv_cstep. }
   intros d ml ? p ? Hpre.
   destruct (rtc_nsteps p) as [n pn].
   inv_csteps pn; simpl in *.
-   left with ml; auto. solve_cnf.
+   left. easy. solve_cnf.
   inv_cstep; eauto.
 Qed.
 
